Auxiliary/Lemmas.dfy
@@ -1,0 +1,59 @@
+include "Set.dfy"
+
+
+lemma mult_preserves_order(a:int, b:int, a':int, b':int)  // Creo que ya no se usa
+  requires 0 <= a <= a'
+  requires 0 <= b <= b'
+  ensures a*b <= a'*b'
+{
+}
+
+
+lemma identity_substraction_lemma<T>(S:set<T>, E:set<T>)
+requires E == {}
+ensures S - E == S
+{}
+
+
+lemma if_smaller_then_less_cardinality<T>(A:set<T>, B:set<T>)
+requires A <= B
+ensures |A| <= |B|
+{
+  if (A == {}) {
+  }
+  else {
+    var a :| a in A && a in B;
+    if_smaller_then_less_cardinality(A - {a}, B - {a});
+  }
+}
+
+
+lemma in_universe_lemma_Set(S:Set, U:Set)
+requires in_universe_Set(S, U)
+ensures S.Size() <= U.Size()
+ensures |S.Model()| <= |U.Model()|
+ensures |S.Universe()| <= |U.Universe()|
+{
+  if_smaller_then_less_cardinality(S.Model(), U.Model());
+  if_smaller_then_less_cardinality(S.Universe(), U.Universe());
+}
+lemma in_universe_lemma_SetSet(S:SetSet, U:SetSet)
+requires in_universe_SetSet(S, U)
+ensures S.Size() <= U.Size()
+ensures |S.Model()| <= |U.Model()|
+ensures |S.Universe()| <= |U.Universe()|
+{
+  if_smaller_then_less_cardinality(S.Model(), U.Model());
+  if_smaller_then_less_cardinality(S.Universe(), U.Universe());
+}
+/*
+lemma in_universe_lemma_SetSetSet(S:SetSetSet, U:SetSetSet)
+requires in_universe_SetSetSet(S, U)
+ensures S.Size() <= U.Size()
+ensures |S.Model()| <= |U.Model()|
+ensures |S.Universe()| <= |U.Universe()|
+{
+  if_smaller_then_less_cardinality(S.Model(), U.Model());
+  if_smaller_then_less_cardinality(S.Universe(), U.Universe());
+}
+*/
