HittingSetToSetCover/HittingSetToSetCover_simple.dfy
@@ -1,0 +1,352 @@
+include "../Problems/HittingSet.dfy"
+include "../Problems/SetCover.dfy"
+include "../Reductions/ReductionHittingSetToSetCover.dfy"
+include "../Auxiliary/Lemmas.dfy"
+
+method HittingSet_to_SetCover_Method(U: set<int>, S: set<set<int>>, k: nat) returns (r:(set<set<int>>, set<set<set<int>>>, nat), ghost counter:nat)
+  requires forall s | s in S ::  s <= U
+  //ensures r == HittingSet_to_SetCover(U, S, k)
+  ensures counter <= poly(U, S, k)
+{
+  counter := 0;
+
+  var newS:set<set<set<int>>> := {};
+  counter := counter + 1;
+  var U' := U;
+  counter := counter + |U|;
+  while (U' != {})
+    decreases |U'|
+    invariant U' <= U
+    invariant newS == (set u | u in (U - U') :: (set s | s in S && u in s))
+    invariant counter <= 1 + |U| + (|U| - |U'|)*(poly_outer_loop(U, S, k) + 1)
+  {
+    counter := counter + 1;
+    U', newS, counter := HittingSet_to_SetCover_outer_loop(U, S, k, U', newS, counter);
+  }
+  counter := counter + 1;
+  identity_substraction_lemma(U, U');
+
+  var S_contains_empty:bool := false;
+  var S' := S;
+  counter := counter + |S|;
+  assert counter <= poly1(U, S, k);
+  while (S' != {})
+    decreases |S'|
+    invariant S' <= S
+    invariant S_contains_empty == ({} in (S - S'))
+    invariant counter <= poly1(U, S, k) + (|S| - |S'|)*(poly_contains_empty_loop(U, S, k) + 1)
+  {
+    counter := counter + 1;
+    S', S_contains_empty, counter := HittingSet_to_SetCover_S_contains_empty_loop(U, S, k, S', S_contains_empty, counter);
+  }
+  assert counter <= poly1(U, S, k) + |S|*(poly_contains_empty_loop(U, S, k) + 1);
+  counter := counter + 1;
+
+  if (S_contains_empty) {
+    var newS := {};
+    counter := counter + 1;
+    var S' := S;
+    counter := counter;
+    //assert counter <= poly1(U, S, k) + |S|*(poly_contains_empty_loop(U, S, k) + 1) + |S| + 1;
+    assert counter <= poly2(U, S, k);
+    while (S' != {})
+      decreases |S'|
+      invariant S' <= S
+      invariant newS == (set s | s in (S - S') :: {s})
+      invariant counter <= poly2(U, S, k) + (|S| - |S'|)*(poly_edge_case_loop(U, S, k) + 1)
+    {
+      counter := counter + 1;
+      S', newS, counter := HittingSet_to_SetCover_edge_case_loop(U, S, k, S', newS, counter);
+      //assert counter <= poly2(U, S, k) + (|S| - |S'| - 1)*(poly_edge_case_loop(U, S, k) + 1) + 1 + 2*|S|*|U| + |U|;
+    }
+    //assert counter <= poly2(U, S, k) + |S|*(poly_edge_case_loop(U, S, k) + 1);
+    counter := counter + 1;
+    assert counter <= poly(U, S, k);
+    return (S, newS, 0), counter;
+  }
+  else {
+    //assert counter <= poly1(U, S, k) + |S|*(|S|*|U| + 2*|U| + 1) + 1;
+    return (S, newS, k), counter;
+  }
+
+}
+
+
+method HittingSet_to_SetCover_outer_loop(U:set<int>, S:set<set<int>>, k:nat, U':set<int>, newS:set<set<set<int>>>, ghost counter_in:nat) returns (U'':set<int>, newS':set<set<set<int>>>, ghost counter:nat)
+// Problem requirements
+requires forall s | s in S ::  s <= U
+// Termination
+requires U' != {}
+// Invariant in
+requires U' <= U
+requires newS == (set u | u in (U - U') :: (set s | s in S && u in s))
+// Decreases
+ensures |U''| == |U'| - 1
+// Invariant out
+ensures U'' <= U
+ensures newS' == (set u | u in (U - U'') :: (set s | s in S && u in s))
+// Counter
+ensures counter <= counter_in + poly_outer_loop(U, S, k) // 2*|S|*|S|*|U| + 2*|S|*|U|*|U| + 5*|S|*|U| + 3*|S| + |U| + 2
+{
+  counter := counter_in;
+  var u :| u in U';
+  counter := counter + 1;
+  U'' := U' - {u};
+  counter := counter + |U|;
+
+  var sets_in_S_that_contain_u:set<set<int>> := {};
+  var S' := S;
+  counter := counter + |S|;
+  while (S' != {})
+    decreases |S'|
+    invariant S' <= S
+    invariant sets_in_S_that_contain_u == (set s | s in (S - S') && u in s)
+    invariant counter <= counter_in + |S| + |U| + 1 + (|S| - |S'|)*(poly_middle_loop(U, S, k) + 1)
+  {
+    counter := counter + 1;
+    S', sets_in_S_that_contain_u, counter := HittingSet_to_SetCover_middle_loop(U, S, k, S', u, sets_in_S_that_contain_u, counter);
+  }
+  counter := counter + 1;
+
+  newS' := newS + {sets_in_S_that_contain_u};
+  counter := counter + |S|*|U|*|U|;
+
+  assert counter <= counter_in + 2*|S|*|S|*|U| + 2*|S|*|U|*|U| + 5*|S|*|U| + 3*|S| + |U| + 2;
+
+  assert newS' == (set v | v in (U - U'') :: (set s | s in S && v in s)) by {
+    assert newS' == (set v | v in (U - U') :: (set s | s in S && v in s)) + {sets_in_S_that_contain_u};
+    assert newS' == (set v | v in (U - U') :: (set s | s in S && v in s)) + {(set s | s in (S - S') && u in s)};
+    assert (S - S') == S;
+    assert newS' == (set v | v in (U - U') + {u} :: (set s | s in S && v in s));
+    assert (U - U'') == (U - U') + {u};
+  }
+  
+}
+
+
+method HittingSet_to_SetCover_middle_loop(U:set<int>, S:set<set<int>>, k:nat, S':set<set<int>>, u:int, sets_in_S_that_contain_u:set<set<int>>, ghost counter_in:nat) returns (S'':set<set<int>>, sets_in_S_that_contain_u':set<set<int>>, ghost counter:nat)
+// Problem requirements
+requires forall s | s in S ::  s <= U
+// Termination
+requires S' != {}
+// Invariant in
+requires S' <= S
+requires sets_in_S_that_contain_u == (set s | s in (S - S') && u in s)
+// Decreases
+ensures |S''| == |S'| - 1
+// Invariant out
+ensures S'' <= S
+ensures sets_in_S_that_contain_u' == (set s | s in (S - S'') && u in s)
+// Counter
+ensures counter <= counter_in + poly_middle_loop(U, S, k)
+{
+  counter := counter_in;
+  sets_in_S_that_contain_u' := sets_in_S_that_contain_u;
+
+  var s :| s in S';
+  counter := counter + |U|;
+  S'' := S' - {s};
+  counter := counter + |S|*|U|;
+
+  var s_contains_u:bool := false;
+  var s' := s;
+  counter := counter + |U|;
+  while (s' != {})
+    decreases |s'|
+    invariant s' <= s
+    invariant s_contains_u == (u in (s - s'))
+    invariant counter == counter_in + |S|*|U| + 2*|U| + (|s| - |s'|)*(|U| + 3)
+  {
+    counter := counter + 1;
+    s', s_contains_u, counter := HittingSet_to_SetCover_inner_loop(U, S, k, s, s', u, s_contains_u, counter);
+  }
+  counter := counter + 1;
+  assert counter <= counter_in + poly3(U, S, k) by {
+    //assert counter <= counter_in + |S|*|U| + 2*|U| + (|s| - |s'|)*(|U| + 3) + 1;
+    if_smaller_then_less_cardinality(s, U);
+    //assert |s| <= |U|;
+    //assert (|s| - |s'|) <= |U|;
+    aux_lemma_1(U, S, k, s, s');
+    //assert (|s| - |s'|)*(|U| + 3) <= (|U|)*(|U| + 3);
+    //assert counter <= counter_in + |S|*|U| + 2*|U| + (|U|)*(|U| + 3) + 1;
+  }
+
+  if (s_contains_u) {
+    sets_in_S_that_contain_u' := sets_in_S_that_contain_u + {s};
+    counter := counter + |S|*|U|;
+  }
+  assert counter <= counter_in + |S|*|U| + poly3(U, S, k);
+  assert counter <= counter_in + poly_middle_loop(U, S, k);
+}
+
+
+method HittingSet_to_SetCover_inner_loop(U:set<int>, S:set<set<int>>, k:nat, s:set<int>, s':set<int>, u:int, s_contains_u:bool, ghost counter_in:nat) returns (s'':set<int>, s_contains_u':bool, ghost counter:nat)
+// Problem requirements
+requires forall s | s in S ::  s <= U
+// Termination
+requires s' != {}
+// Invariant in
+requires s' <= s
+requires s_contains_u == (u in (s - s'))
+// Decreases
+ensures |s''| == |s'| - 1
+// Invariant out
+ensures s'' <= s
+ensures s_contains_u' == (u in (s - s''))
+// Counter
+ensures counter == counter_in + poly_inner_loop(U, S, k)
+{
+  counter := counter_in;
+  s_contains_u' := s_contains_u;
+
+  var e :| e in s';
+  counter := counter + 1;
+  s'' := s' - {e};
+  counter := counter + |U|;
+
+  if (e == u) {
+    s_contains_u' := true;
+  }
+  counter := counter + 1;
+}
+
+
+method HittingSet_to_SetCover_S_contains_empty_loop(U:set<int>, S:set<set<int>>, k:nat, S':set<set<int>>, S_contains_empty:bool, ghost counter_in:nat) returns (S'':set<set<int>>, S_contains_empty':bool, ghost counter:nat)
+// Problem requirements
+requires forall s | s in S ::  s <= U
+// Termination
+requires S' != {}
+// Invariant in
+requires S' <= S
+requires S_contains_empty == ({} in (S - S'))
+// Decreases
+ensures |S''| == |S'| - 1
+// Invariant out
+ensures S'' <= S
+ensures S_contains_empty'== ({} in (S - S''))
+// Counter
+ensures counter == counter_in + poly_contains_empty_loop(U, S, k)
+{
+  counter := counter_in;
+  S_contains_empty' := S_contains_empty;
+
+  var s :| s in S';
+  counter := counter + |U|;
+  S'' := S' - {s};
+  counter := counter + |S|*|U|;
+  if (s == {}) {
+    S_contains_empty' := true;
+  }
+  counter := counter + |U|;
+}
+
+
+method HittingSet_to_SetCover_edge_case_loop(U:set<int>, S:set<set<int>>, k:nat, S':set<set<int>>, newS:set<set<set<int>>>, ghost counter_in:nat) returns (S'':set<set<int>>, newS':set<set<set<int>>>, ghost counter:nat)
+// Problem requirements
+requires forall s | s in S ::  s <= U
+// Termination
+requires S' != {}
+// Invariant in
+requires S' <= S
+requires newS == (set s | s in (S - S') :: {s})
+// Decreases
+ensures |S''| == |S'| - 1
+// Invariant out
+ensures S'' <= S
+ensures newS' == (set s | s in (S - S'') :: {s})
+// Counter
+ensures counter == counter_in + poly_edge_case_loop(U, S, k)     //2*|S|*|U| + |U|
+{
+  counter := counter_in;
+  var s :| s in S';
+  counter := counter + |U|;
+  S'' := S' - {s};
+  counter := counter + |S|*|U|;
+  newS' := newS + {{s}};
+  counter := counter + |S|*|U|;
+}
+
+/*
+const c:nat := 100
+
+ghost function O_SSU_SUU(U: set<int>, S: set<set<int>>, k: nat) : (o:nat) {
+  c*|S|*|S|*|U| + c*|S|*|U|*|U| + c*|S|*|U| + c*|S| + c*|U| + c
+}
+
+ghost function O_SSUU_SUUU(U: set<int>, S: set<set<int>>, k: nat) : (o:nat) {
+  c*|S|*|S|*|U|*|U| + c*|S|*|U|*|U|*|U| + c*|S|*|S|*|U| + c*|S|*|U|*|U| + c*|S|*|U| + c*|U|*|U| + c*|S| + c*|U| + c
+}
+*/
+
+ghost function poly1(U: set<int>, S: set<set<int>>, k: nat) : (o:nat)
+ensures |S| + |U|*(poly_outer_loop(U, S, k) + 2) + 2 <= o
+{
+  2*|S|*|S|*|U|*|U| + 2*|S|*|U|*|U|*|U| + 5*|S|*|U|*|U| + 3*|S|*|U| + |U|*|U| + |S| + 4*|U| + 2
+}
+
+ghost function poly2(U: set<int>, S: set<set<int>>, k: nat) : (o:nat)
+ensures poly1(U, S, k) + |S|*(poly_contains_empty_loop(U, S, k) + 1) + |S| + 1 <= o
+{
+  2*|S|*|S|*|U|*|U| + 2*|S|*|U|*|U|*|U| + |S|*|S|*|U| + 5*|S|*|U|*|U| + 5*|S|*|U| + |U|*|U| + 3*|S| + 4*|U| + 4
+}
+
+ghost function poly3(U: set<int>, S: set<set<int>>, k: nat) : (o:nat)
+{
+  |S|*|U| + 2*|U| + (|U|)*(|U| + 3) + 1
+}
+
+ghost function poly_inner_loop(U: set<int>, S: set<set<int>>, k: nat) : (o:nat)
+{
+  |U| + 2
+}
+
+ghost function poly_middle_loop(U: set<int>, S: set<set<int>>, k: nat) : (o:nat)
+  ensures |S|*|U| + poly3(U, S, k) <= o
+{
+  2*|S|*|U| + 2*|U| + |U|*(|U| + 3) + 1
+}
+
+ghost function poly_outer_loop(U: set<int>, S: set<set<int>>, k: nat) : (o:nat)
+{
+  2*|S|*|S|*|U| + 2*|S|*|U|*|U| + 5*|S|*|U| + 3*|S| + |U| + 2
+}
+
+ghost function poly_contains_empty_loop(U: set<int>, S: set<set<int>>, k: nat) : (o:nat)
+{
+  |S|*|U| + 2*|U|
+}
+
+ghost function poly_edge_case_loop(U: set<int>, S: set<set<int>>, k: nat) : (o:nat)
+{
+  2*|S|*|U| + |U|
+}
+
+ghost function poly(U: set<int>, S: set<set<int>>, k: nat) : (o:nat)
+  //ensures poly1(U, S, k) + |S|*(|S|*|U| + 2*|U| + 1) + 1 <= o
+  ensures poly2(U, S, k) + |S|*(poly_edge_case_loop(U, S, k) + 1) + 1 <= o
+{
+  /*
+  calc == {
+    poly1(U, S, k) + |S|*(|S|*|U| + 2*|U| + 1) + 1;
+    poly1(U, S, k) + |S|*|S|*|U| + 2*|S|*|U| + |S| + 1;
+  }
+  */
+
+  calc == {
+    poly2(U, S, k) + |S|*(poly_edge_case_loop(U, S, k) + 1) + 1;
+    poly2(U, S, k) + |S|*(2*|S|*|U| + |U| + 1) + 1;
+    poly2(U, S, k) + 2*|S|*|S|*|U| + |S|*|U| + |S| + 1;
+    poly2(U, S, k) + 2*|S|*|S|*|U| + |S|*|U| + |S| + 1;
+    (2*|S|*|S|*|U|*|U| + 2*|S|*|U|*|U|*|U| + |S|*|S|*|U| + 5*|S|*|U|*|U| + 5*|S|*|U| + |U|*|U| + 3*|S| + 4*|U| + 4) + 2*|S|*|S|*|U| + |S|*|U| + |S| + 1;
+    2*|S|*|S|*|U|*|U| + 2*|S|*|U|*|U|*|U| + 3*|S|*|S|*|U| + 5*|S|*|U|*|U| + 6*|S|*|U| + |U|*|U| + 4*|S| + 4*|U| + 5;
+  }
+
+  2*|S|*|S|*|U|*|U| + 2*|S|*|U|*|U|*|U| + 3*|S|*|S|*|U| + 5*|S|*|U|*|U| + 6*|S|*|U| + |U|*|U| + 4*|S| + 4*|U| + 5
+
+}
+
+lemma aux_lemma_1(U: set<int>, S: set<set<int>>, k: nat, s: set<int>, s': set<int>)
+requires 0 <= |s'| <= |s| <= |U|
+ensures (|s| - |s'|)*(|U| + 3) <= (|U|)*(|U| + 3)
+{
+}
