VerificationSetCover/VerificationSetCover_types.dfy
@@ -1,0 +1,258 @@
+include "../Problems/SetCover.dfy"
+include "../Auxiliary/Set.dfy"
+include "../Auxiliary/Lemmas.dfy"
+
+
+method verifySetCover(U:Set<int>, S:SetSet<int>, k:nat, I:SetSet<int>) returns (b:bool, ghost counter:nat)   
+requires forall s | s in S.Model() :: s <= U.Model()
+
+requires init_Set(U)
+requires init_SetSet(S)
+requires init_SetSet(I)
+requires |U.Model()| == S.maximumSizeElements()
+
+ensures b == (I.Model() <= S.Model() && isCover(U.Model(), I.Model()) && |I.Model()| <= k)
+ensures counter <= poly(U, S, k, I)
+{
+  counter := 0;
+
+  var I_cardinality:int;
+  I_cardinality, counter := I.Cardinality(counter);
+  var I_seq_S:bool;
+  I_seq_S, counter := isSubset(I, S, counter);
+
+  if (!(I_seq_S && I_cardinality <= k)) {
+    return false, counter;
+  }
+
+  var U':Set<int>;
+  U', counter := U.Copy(counter);
+  b := true;
+  var U'_empty:bool;
+  U'_empty, counter := U'.Empty(counter);
+
+  assert counter <= poly_isSubset(I, S) + U.Size() + 2*constant;
+
+  while (!U'_empty && b)
+    // Termination
+    decreases |U'.Model()|
+    invariant U'_empty == (U'.Model() == {})
+    // Types
+    invariant in_universe_Set(U', U)
+    invariant in_universe_SetSet(I, S)
+    invariant correct_Set(U')
+    // Regular invariants
+    invariant b == isCover(U.Model() - U'.Model() , I.Model())
+    // Counter
+    invariant counter <= poly_isSubset(I, S) + U.Size() + 2*constant + (|U.Model()| - |U'.Model()|)*poly_outer_loop(U, S, k)
+  {
+    b, U', U'_empty, counter := verifySetCover_outer_loop(U, S, k, I, U', counter);
+  }
+  assert b ==> U.Model() - U'.Model() == U.Model();
+  assert counter <= poly(U, S, k, I);
+
+  b := b;
+}
+
+
+method isSubset(S1:SetSet<int>, S2:SetSet<int>, ghost counter_in:nat) returns (b:bool, ghost counter:nat)
+requires correct_SetSet(S1)
+requires correct_SetSet(S2)
+ensures b == (S1.Model() <= S2.Model())
+ensures counter <= counter_in + poly_isSubset(S1, S2)
+{
+  counter := counter_in;
+  b := true;
+  var S1';
+  S1', counter := S1.Copy(counter);
+  var S1'_empty:bool;
+  S1'_empty, counter := S1'.Empty(counter);
+  
+  while (!S1'_empty)
+  // Termination
+  decreases |S1'.Model()|
+  invariant S1'_empty == (S1'.Model() == {})
+  // Types
+  invariant correct_SetSet(S1')
+  invariant in_universe_SetSet(S1', S1)
+  // Regular invariants
+  invariant b == ((S1.Model() - S1'.Model()) <= S2.Model())
+  // Counter
+  invariant counter <= counter_in + S1.Size() + constant + (|S1.Model()| - |S1'.Model()|)*(poly_isSubset_loop(S1, S2))
+  {
+    S1', S1'_empty, b, counter := isSubset_loop(S1, S2, S1', counter, b);
+  }
+}
+
+
+method isSubset_loop(S1:SetSet<int>, S2:SetSet<int>, S1':SetSet<int>, ghost counter_in:nat, b:bool) returns (S1'':SetSet<int>, S1'_empty:bool, b':bool, ghost counter:nat)
+// Termination in
+requires S1'.Model() != {}
+// Types in
+requires in_universe_SetSet(S1', S1)
+requires correct_SetSet(S2)
+// Invariant in
+requires b == ((S1.Model() - S1'.Model()) <= S2.Model())
+// Termination out
+ensures |S1''.Model()| == |S1'.Model()| - 1
+ensures S1'_empty == (S1''.Model() == {})
+// Types out
+ensures correct_SetSet(S1'')
+ensures in_universe_SetSet(S1'', S1)
+// Invariant out
+ensures b' == ((S1.Model() - S1''.Model()) <= S2.Model())
+// Counter
+ensures counter <= counter_in + poly_isSubset_loop(S1, S2)
+{
+  in_universe_lemma_SetSet(S1', S1);
+
+  counter := counter_in;
+  var s:Set<int>;
+  s, counter := S1'.Pick(counter);
+
+  var s_in_S2:bool;
+  s_in_S2, counter := S2.Contains(s, counter);
+  b' := b && s_in_S2;
+
+  S1'', counter := S1'.Remove(s, counter);
+  S1'_empty, counter := S1''.Empty(counter);
+}
+
+
+
+method verifySetCover_outer_loop(U:Set<int>, S:SetSet<int>, k:nat, I:SetSet<int>, U':Set<int>, ghost counter_in:nat) returns (b1:bool, U'':Set<int>, U''_empty:bool, ghost counter:nat)
+// Termination in
+requires U'.Model() != {}
+// Types in
+requires correct_Set(U)
+requires correct_Set(U')
+requires correct_SetSet(S)
+requires correct_SetSet(I)
+requires in_universe_Set(U', U)
+requires in_universe_SetSet(I, S)
+// Invariant in
+requires isCover(U.Model() - U'.Model(), I.Model())
+// Termination out
+ensures |U''.Model()| == |U'.Model()| - 1
+ensures U''_empty == (U''.Model() == {})
+// Types out
+ensures correct_Set(U'')
+ensures in_universe_Set(U'', U)
+// Invariant out
+ensures b1 == isCover(U.Model() - U''.Model(), I.Model())
+// Counter
+ensures counter <= counter_in + poly_outer_loop(U, S, k)
+{
+  in_universe_lemma_Set(U', U);
+  in_universe_lemma_SetSet(I, S);
+
+  counter := counter_in;
+  var u:int;
+  u, counter := U'.Pick(counter);
+  U'', counter := U'.Remove(u, counter);
+
+  var I':SetSet<int>;
+  I', counter := I.Copy(counter);
+
+  var b2:bool := false;
+  var I'_empty:bool;
+  I'_empty, counter := I'.Empty(counter);
+  assert counter <= counter_in + 2*constant + U.Size() + S.Size();
+  while (!I'_empty && !b2)
+    // Termination
+    decreases |I'.Model()|
+    invariant I'_empty == (I'.Model() == {})
+    // Types
+    invariant correct_SetSet(I')
+    invariant in_universe_SetSet(I, S)
+    invariant in_universe_SetSet(I', I)
+    // Regular invariants
+    invariant b2 == (exists i' | i' in I.Model() - I'.Model() :: u in i')
+    // Counter
+    invariant counter <= counter_in + 2*constant + U.Size() + S.Size() + (|I.Model()|-|I'.Model()|)*(poly_inner_loop(U, S, k) + constant)
+  {
+    b2, I', I'_empty, counter := verifySetCover_inner_loop(U, S, k, I, I', u, counter);
+  }
+  b1 := b2;
+
+  U''_empty, counter := U''.Empty(counter);
+
+  assert U.Model() - U''.Model() == U.Model() - U'.Model() + {u};
+  assert counter <= counter_in + 3*constant + U.Size() + S.Size() + (|S.Model()|)*(poly_inner_loop(U, S, k) + constant) by {
+    assert counter <= counter_in + 3*constant + U.Size() + S.Size() + (|I.Model()|)*(poly_inner_loop(U, S, k) + constant);
+  }
+  assert counter <= counter_in + poly_outer_loop(U, S, k);
+}
+
+
+
+method verifySetCover_inner_loop(U:Set<int>, S:SetSet<int>, k:nat, I:SetSet<int>, I':SetSet<int>, u:int, ghost counter_in:nat) returns (b2:bool, I'':SetSet<int>, I''_empty:bool, ghost counter:nat)
+// Termination in
+requires I'.Model() != {}
+// Types in
+requires correct_Set(U)
+requires in_universe_SetSet(I, S)
+requires in_universe_SetSet(I', I)
+// Invariant in
+requires !(exists i' | i' in I.Model() - I'.Model() :: u in i')
+// Termination out
+ensures |I''.Model()| == |I'.Model()| - 1
+ensures I''_empty == (I''.Model() == {})
+// Types out
+ensures correct_SetSet(I'')
+ensures in_universe_SetSet(I'', I)
+// Invariant out
+ensures b2 == (exists i' | i' in I.Model() - I''.Model() :: u in i')
+// Counter
+ensures counter <= counter_in + poly_inner_loop(U, S, k)
+{
+  in_universe_lemma_SetSet(I', I);
+  in_universe_lemma_SetSet(I, S);
+
+  counter := counter_in;
+  var i:Set<int>;
+  i, counter := I'.Pick(counter);
+  b2, counter := i.Contains(u, counter);
+  I'', counter := I'.Remove(i, counter);
+  I''_empty, counter := I''.Empty(counter);
+}
+
+
+
+ghost function poly_inner_loop(U:Set<int>, S:SetSet<int>, k:nat) : (o:nat)
+{
+  S.Size() + 2*S.maximumSizeElements() + constant
+}
+ghost function poly_outer_loop(U:Set<int>, S:SetSet<int>, k:nat) : (o:nat)
+{
+  3*constant + U.Size() + S.Size() + |S.Model()|*poly_inner_loop(U, S, k) + constant*|S.Model()|
+}
+ghost function poly_isSubset_loop(S1:SetSet<int>, S2:SetSet<int>) : (o:nat)
+{
+  S1.Size() + S2.Size() + S1.maximumSizeElements() + constant
+}
+ghost function poly_isSubset(S1:SetSet<int>, S2:SetSet<int>) : (o:nat)
+{
+  (|S1.Model()| + constant)*S1.Size() + |S1.Model()|*S2.Size() + |S1.Model()|*S1.maximumSizeElements() + |S1.Model()| + constant
+}
+
+ghost function poly(U:Set<int>, S:SetSet<int>, k:nat, I:SetSet<int>) : (o:nat)
+ensures poly_isSubset(I, S) + U.Size() + 2*constant + |U.Model()|*poly_outer_loop(U, S, k) <= o
+{
+  assert poly_outer_loop(U, S, k) == (3*constant + U.Size() + S.Size() + |S.Model()|*poly_inner_loop(U, S, k) + constant*|S.Model()|);
+  assert poly_inner_loop(U, S, k) == S.Size() + 2*S.maximumSizeElements() + constant;
+  assert poly_isSubset(I, S) == (|I.Model()| + constant)*I.Size() + |I.Model()|*S.Size() + |I.Model()|*I.maximumSizeElements() + |I.Model()| + constant;
+  calc == {
+    poly_isSubset(I, S) + U.Size() + 2*constant + |U.Model()|*poly_outer_loop(U, S, k);
+    poly_isSubset(I, S) + U.Size() + 2*constant + |U.Model()|*(3*constant + U.Size() + S.Size() + |S.Model()|*poly_inner_loop(U, S, k) + constant*|S.Model()|);
+    poly_isSubset(I, S) + U.Size() + 2 + 3*|U.Model()| + |U.Model()|*U.Size() + |U.Model()|*S.Size() + |U.Model()|*|S.Model()|*poly_inner_loop(U, S, k) + |U.Model()|*|S.Model()|;
+    poly_isSubset(I, S) + U.Size() + 2 + 3*|U.Model()| + |U.Model()|*U.Size() + |U.Model()|*S.Size() + |U.Model()|*|S.Model()|*(S.Size() + 2*S.maximumSizeElements() + constant) + |U.Model()|*|S.Model()|;
+    poly_isSubset(I, S) + U.Size() + 2 + 3*|U.Model()| + |U.Model()|*U.Size() + |U.Model()|*S.Size() + |U.Model()|*|S.Model()|*S.Size() + 2*|U.Model()|*|S.Model()|*S.maximumSizeElements() + |U.Model()|*|S.Model()| + |U.Model()|*|S.Model()|;
+    poly_isSubset(I, S) + |U.Model()|*|S.Model()|*S.Size() + 2*|U.Model()|*|S.Model()|*S.maximumSizeElements() + |U.Model()|*U.Size() + |U.Model()|*S.Size() + 2*|U.Model()|*|S.Model()| + U.Size() + 3*|U.Model()| + 2*constant;
+    (|I.Model()| + constant)*I.Size() + |I.Model()|*S.Size() + |I.Model()|*I.maximumSizeElements() + |I.Model()| + |U.Model()|*|S.Model()|*S.Size() +
+    2*|U.Model()|*|S.Model()|*S.maximumSizeElements() + |U.Model()|*U.Size() + |U.Model()|*S.Size() + 2*|U.Model()|*|S.Model()| + U.Size() + 3*|U.Model()| + 3*constant;
+  }
+  
+  (|I.Model()| + constant)*I.Size() + |I.Model()|*S.Size() + |I.Model()|*I.maximumSizeElements() + |I.Model()| + |U.Model()|*|S.Model()|*S.Size() +
+    2*|U.Model()|*|S.Model()|*S.maximumSizeElements() + |U.Model()|*U.Size() + |U.Model()|*S.Size() + 2*|U.Model()|*|S.Model()| + U.Size() + 3*|U.Model()| + 3*constant
+}
